# Review for Exam IV - MATE3001
## Practice Problems with Step-by-Step Solutions

---

## Part I: Multiple Choice Practice

### Problem 1: Domain of a Rational Expression
Find the domain of the expression $\dfrac{x-2}{x^2-16}$

**Step-by-Step Solution:**
1. Identify restrictions: The denominator cannot equal zero
2. Set denominator equal to zero: $x^2 - 16 = 0$
3. Factor: $(x-4)(x+4) = 0$
4. Solve: $x = 4$ or $x = -4$
5. **Domain:** $\{x | x \neq \pm 4\}$

---

### Problem 2: Simplifying Rational Expressions
Simplify $\dfrac{x^2-9}{x^2+6x+9}$

**Step-by-Step Solution:**
1. Factor the numerator: $x^2 - 9 = (x-3)(x+3)$
2. Factor the denominator: $x^2 + 6x + 9 = (x+3)(x+3) = (x+3)^2$
3. Write factored form: $\dfrac{(x-3)(x+3)}{(x+3)^2}$
4. Cancel common factors: $\dfrac{x-3}{x+3}$
5. **Answer:** $\dfrac{x-3}{x+3}$

---

### Problem 3: Multiplying Rational Expressions
Simplify $\dfrac{x^2-4}{x+3} \cdot \dfrac{x+3}{x+2}$

**Step-by-Step Solution:**
1. Factor $x^2-4$: $(x-2)(x+2)$
2. Write as: $\dfrac{(x-2)(x+2)}{x+3} \cdot \dfrac{x+3}{x+2}$
3. Multiply: $\dfrac{(x-2)(x+2)(x+3)}{(x+3)(x+2)}$
4. Cancel $(x+3)$ and $(x+2)$: $x-2$
5. **Answer:** $x-2$

---

### Problem 4: Simplifying Radicals
Simplify $\sqrt{98}$

**Step-by-Step Solution:**
1. Find perfect square factors: $98 = 49 \times 2$
2. Separate: $\sqrt{98} = \sqrt{49 \times 2}$
3. Simplify: $\sqrt{49} \times \sqrt{2} = 7\sqrt{2}$
4. **Answer:** $7\sqrt{2}$

---

### Problem 5: Rationalizing Denominators
Rationalize $\dfrac{5}{\sqrt{7}}$

**Step-by-Step Solution:**
1. Multiply by $\dfrac{\sqrt{7}}{\sqrt{7}}$: $\dfrac{5}{\sqrt{7}} \cdot \dfrac{\sqrt{7}}{\sqrt{7}}$
2. Simplify numerator: $5\sqrt{7}$
3. Simplify denominator: $\sqrt{7} \cdot \sqrt{7} = 7$
4. **Answer:** $\dfrac{5\sqrt{7}}{7}$

---

### Problem 6: Combining Radical Expressions
Simplify $3\sqrt{18} - 2\sqrt{8} + \sqrt{32}$

**Step-by-Step Solution:**
1. Simplify each radical:
   - $\sqrt{18} = \sqrt{9 \times 2} = 3\sqrt{2}$
   - $\sqrt{8} = \sqrt{4 \times 2} = 2\sqrt{2}$
   - $\sqrt{32} = \sqrt{16 \times 2} = 4\sqrt{2}$
2. Substitute: $3(3\sqrt{2}) - 2(2\sqrt{2}) + 4\sqrt{2}$
3. Multiply: $9\sqrt{2} - 4\sqrt{2} + 4\sqrt{2}$
4. Combine like terms: $(9 - 4 + 4)\sqrt{2} = 9\sqrt{2}$
5. **Answer:** $9\sqrt{2}$

---

### Problem 7: Solving Rational Equations
Solve $\dfrac{4}{x} + \dfrac{3}{x-2} = 1$

**Step-by-Step Solution:**
1. Find LCD: $x(x-2)$
2. Multiply all terms by LCD: $x(x-2) \cdot \dfrac{4}{x} + x(x-2) \cdot \dfrac{3}{x-2} = x(x-2) \cdot 1$
3. Simplify: $4(x-2) + 3x = x(x-2)$
4. Expand: $4x - 8 + 3x = x^2 - 2x$
5. Combine: $7x - 8 = x^2 - 2x$
6. Rearrange: $0 = x^2 - 9x + 8$
7. Factor: $0 = (x-1)(x-8)$
8. Solve: $x = 1$ or $x = 8$
9. **Answer:** $x = 1$ or $x = 8$

---

### Problem 8: Identifying Functions
Which of the following relations is **NOT** a function?

A) $\{(2,3), (3,4), (4,5), (5,6)\}$
B) $\{(1,5), (1,7), (3,9)\}$
C) $\{(2,3), (3,3), (4,3), (5,3)\}$
D) $f(x) = x^2 + 1$

**Step-by-Step Solution:**
1. Recall: A relation is a function if each input has exactly one output
2. Check option A: All inputs different ✓
3. Check option B: Input 1 appears twice with different outputs (3 and 7) ✗
4. Check option C: All inputs different ✓
5. Check option D: Functions always pass the definition ✓
6. **Answer:** Option B is NOT a function

---

### Problem 9: Intercepts of Linear Functions
For the function $f(x) = 2x - 8$, find the $y$-intercept as an ordered pair.

**Step-by-Step Solution:**
1. Recall: The $y$-intercept occurs when $x = 0$
2. Substitute: $f(0) = 2(0) - 8$
3. Simplify: $f(0) = -8$
4. Write as ordered pair: $(0, -8)$
5. **Answer:** $(0, -8)$

---

### Problem 10: Conjugates
Find the conjugate of $3 + \sqrt{11}$

**Step-by-Step Solution:**
1. Recall: The conjugate of $a + \sqrt{b}$ is $a - \sqrt{b}$
2. Apply: The conjugate of $3 + \sqrt{11}$ is $3 - \sqrt{11}$
3. **Answer:** $3 - \sqrt{11}$

---

### Problem 11: Exponential to Radical Form
Write $x^{5/3}$ in radical form.

**Step-by-Step Solution:**
1. Recall: $x^{m/n} = \sqrt[n]{x^m}$
2. Identify: $m = 5$ and $n = 3$
3. Apply: $x^{5/3} = \sqrt[3]{x^5}$
4. **Answer:** $\sqrt[3]{x^5}$

---

### Problem 12: Radical to Exponential Form
Write $\sqrt[4]{x^3}$ in exponential notation.

**Step-by-Step Solution:**
1. Recall: $\sqrt[n]{x^m} = x^{m/n}$
2. Identify: $m = 3$ and $n = 4$
3. Apply: $\sqrt[4]{x^3} = x^{3/4}$
4. **Answer:** $x^{3/4}$

---

## Part II: Development Problems

### Problem 13: Simplifying Rational Expressions
Simplify completely: $\dfrac{x^2+3x-10}{x^2-25}$

**Step-by-Step Solution:**
1. Factor the numerator: $x^2 + 3x - 10$
   - Find two numbers that multiply to $-10$ and add to $3$: $5$ and $-2$
   - $x^2 + 3x - 10 = (x+5)(x-2)$

2. Factor the denominator: $x^2 - 25$
   - Difference of squares: $(x-5)(x+5)$

3. Write factored form:
   $$\dfrac{(x+5)(x-2)}{(x-5)(x+5)}$$

4. Cancel common factor $(x+5)$:
   $$\dfrac{x-2}{x-5}$$

5. **Final Answer:** $\dfrac{x-2}{x-5}$

---

### Problem 14: Dividing Rational Expressions
Perform the division and simplify: $\dfrac{x^2-16}{x^2+3x-10} \div \dfrac{x-4}{x+5}$

**Step-by-Step Solution:**
1. Rewrite division as multiplication by reciprocal:
   $$\dfrac{x^2-16}{x^2+3x-10} \cdot \dfrac{x+5}{x-4}$$

2. Factor all expressions:
   - $x^2 - 16 = (x-4)(x+4)$ (difference of squares)
   - $x^2 + 3x - 10 = (x+5)(x-2)$ (factors: $5$ and $-2$)

3. Substitute factored forms:
   $$\dfrac{(x-4)(x+4)}{(x+5)(x-2)} \cdot \dfrac{x+5}{x-4}$$

4. Multiply:
   $$\dfrac{(x-4)(x+4)(x+5)}{(x+5)(x-2)(x-4)}$$

5. Cancel common factors $(x-4)$ and $(x+5)$:
   $$\dfrac{x+4}{x-2}$$

6. **Final Answer:** $\dfrac{x+4}{x-2}$

---

### Problem 15: Adding Rational Expressions
Perform the addition and simplify: $\dfrac{2}{x-3} + \dfrac{5}{x+2}$

**Step-by-Step Solution:**
1. Find the LCD: $(x-3)(x+2)$

2. Rewrite each fraction with LCD:
   $$\dfrac{2(x+2)}{(x-3)(x+2)} + \dfrac{5(x-3)}{(x-3)(x+2)}$$

3. Expand numerators:
   $$\dfrac{2x+4}{(x-3)(x+2)} + \dfrac{5x-15}{(x-3)(x+2)}$$

4. Add numerators:
   $$\dfrac{2x+4+5x-15}{(x-3)(x+2)}$$

5. Combine like terms:
   $$\dfrac{7x-11}{(x-3)(x+2)}$$

6. Check if numerator can be factored: $7x - 11$ cannot be factored further

7. **Final Answer:** $\dfrac{7x-11}{(x-3)(x+2)}$ or $\dfrac{7x-11}{x^2-x-6}$

---

### Problem 16: Simplifying Radicals with Variables
Simplify completely (assume all variables are positive): $\sqrt{128x^5y^4}$

**Step-by-Step Solution:**
1. Break down into prime factors and perfect squares:
   $$\sqrt{128x^5y^4} = \sqrt{64 \cdot 2 \cdot x^4 \cdot x \cdot y^4}$$

2. Group perfect squares:
   $$\sqrt{64 \cdot x^4 \cdot y^4 \cdot 2 \cdot x}$$

3. Apply property $\sqrt{ab} = \sqrt{a} \cdot \sqrt{b}$:
   $$\sqrt{64} \cdot \sqrt{x^4} \cdot \sqrt{y^4} \cdot \sqrt{2x}$$

4. Simplify each perfect square:
   - $\sqrt{64} = 8$
   - $\sqrt{x^4} = x^2$
   - $\sqrt{y^4} = y^2$

5. Combine:
   $$8x^2y^2\sqrt{2x}$$

6. **Final Answer:** $8x^2y^2\sqrt{2x}$

---

### Problem 17: Solving Rational Equations
Solve the equation and verify your solution: $\dfrac{4}{x-3} - \dfrac{2}{x} = 1$

**Step-by-Step Solution:**
1. Find LCD: $x(x-3)$

2. Multiply all terms by LCD:
   $$x(x-3) \cdot \dfrac{4}{x-3} - x(x-3) \cdot \dfrac{2}{x} = x(x-3) \cdot 1$$

3. Simplify:
   $$4x - 2(x-3) = x(x-3)$$

4. Expand left side:
   $$4x - 2x + 6 = x^2 - 3x$$

5. Combine like terms:
   $$2x + 6 = x^2 - 3x$$

6. Rearrange to standard form:
   $$0 = x^2 - 5x - 6$$

7. Factor:
   $$0 = (x-6)(x+1)$$

8. Solve:
   $$x = 6 \text{ or } x = -1$$

9. **Verify $x = 6$:**
   $$\dfrac{4}{6-3} - \dfrac{2}{6} = \dfrac{4}{3} - \dfrac{1}{3} = \dfrac{3}{3} = 1$$ ✓

10. **Verify $x = -1$:**
    $$\dfrac{4}{-1-3} - \dfrac{2}{-1} = \dfrac{4}{-4} - (-2) = -1 + 2 = 1$$ ✓

11. **Final Answer:** $x = 6$ or $x = -1$

---

### Problem 18: Rationalizing with Conjugates
Rationalize the denominator and simplify: $\dfrac{8}{4-\sqrt{3}}$

**Step-by-Step Solution:**
1. Identify the conjugate of denominator: $4 + \sqrt{3}$

2. Multiply numerator and denominator by conjugate:
   $$\dfrac{8}{4-\sqrt{3}} \cdot \dfrac{4+\sqrt{3}}{4+\sqrt{3}}$$

3. Multiply numerator:
   $$8(4+\sqrt{3}) = 32 + 8\sqrt{3}$$

4. Multiply denominator using $(a-b)(a+b) = a^2 - b^2$:
   $$(4-\sqrt{3})(4+\sqrt{3}) = 16 - 3 = 13$$

5. Write result:
   $$\dfrac{32 + 8\sqrt{3}}{13}$$

6. This can also be written as:
   $$\dfrac{32}{13} + \dfrac{8\sqrt{3}}{13}$$

7. **Final Answer:** $\dfrac{32 + 8\sqrt{3}}{13}$

---

### Problem 19: Function Evaluation
Given the function $f(x) = x^2 - 3x + 5$:

#### Part a) Evaluate $f(-3)$

**Step-by-Step Solution:**
1. Substitute $x = -3$ into the function:
   $$f(-3) = (-3)^2 - 3(-3) + 5$$

2. Calculate $(-3)^2$:
   $$f(-3) = 9 - 3(-3) + 5$$

3. Calculate $-3(-3)$:
   $$f(-3) = 9 + 9 + 5$$

4. Add:
   $$f(-3) = 23$$

5. **Answer:** $f(-3) = 23$

#### Part b) Find $f(a+2)$

**Step-by-Step Solution:**
1. Substitute $x = a+2$ into the function:
   $$f(a+2) = (a+2)^2 - 3(a+2) + 5$$

2. Expand $(a+2)^2$ using $(a+b)^2 = a^2 + 2ab + b^2$:
   $$f(a+2) = a^2 + 4a + 4 - 3(a+2) + 5$$

3. Distribute $-3$:
   $$f(a+2) = a^2 + 4a + 4 - 3a - 6 + 5$$

4. Combine like terms:
   - $a^2$ term: $a^2$
   - $a$ terms: $4a - 3a = a$
   - Constants: $4 - 6 + 5 = 3$

5. Simplify:
   $$f(a+2) = a^2 + a + 3$$

6. **Answer:** $f(a+2) = a^2 + a + 3$

---

## Summary of Key Concepts

### Rational Expressions
- Find domain by setting denominator ≠ 0
- Simplify by factoring and canceling common factors
- Multiply: multiply numerators and denominators, then simplify
- Divide: multiply by reciprocal
- Add/Subtract: find LCD, create equivalent fractions, combine

### Radicals
- Simplify by extracting perfect square factors
- Rationalize denominators (use conjugates for binomials)
- Combine like radicals (same radicand and index)
- Convert between radical and exponential forms: $\sqrt[n]{x^m} = x^{m/n}$

### Solving Rational Equations
1. Find LCD of all fractions
2. Multiply all terms by LCD
3. Solve resulting polynomial equation
4. Check solutions in original equation

### Functions
- Vertical line test: each input has exactly one output
- Evaluate by substituting values
- Find intercepts: $y$-intercept when $x=0$, $x$-intercept when $y=0$

---

**End of Review**
